

Formula Sheet

Equations and Inequalities:

Binomial powers: $(a+b)^2 = a^2 + 2ab + b^2$, $(a+b)^3 = a^3 + 3a^2b + 3ab^2 + b^3$

Difference of squares: $a^2 - b^2 = (a-b)(a+b)$

Difference of cubes: $a^3 - b^3 = (a-b)(a^2 + ab + b^2)$

Sum of cubes: $a^3 + b^3 = (a+b)(a^2 - ab + b^2)$

Difference of n -th powers: $a^n - b^n = (a-b)(a^{n-1} + a^{n-2}b + \dots + b^{n-1})$

Quadratic equation, completing the square: $ax^2 + bx + c = a\left(x + \frac{b}{2a}\right)^2 - \frac{b^2}{4a} + c = 0$

Roots of a quadratic equation: If $b^2 - 4ac \geq 0$ then $x_{1,2} = \frac{-b \pm \sqrt{b^2 - 4ac}}{2a}$.

Factorization: If roots x_1 and x_2 exist then $ax^2 + bx + c = a(x - x_1)(x - x_2)$.

The graph of $y = ax^2 + bx + c$ is called a parabola.

The vertex of a parabola is at the point (x_0, y_0) , where: $x_0 = -\frac{b}{2a}$, $y_0 = -\frac{b^2}{4a} + c$.

Powers and Logarithms:

$a^n \cdot a^m = a^{n+m}$, $a^{-n} = \frac{1}{a^n}$, $\frac{a^m}{a^n} = a^{m-n}$, $\sqrt[n]{a} = a^{\left(\frac{1}{n}\right)}$, $(a^n)^m = a^{n \cdot m}$, $(a \cdot b)^n = a^n \cdot b^n$, $\left(\frac{a}{b}\right)^n = \frac{a^n}{b^n}$.

Definition of logarithm: If $a^x = b$ then $x = \log_a b$. a is the **base** of the logarithm.

Change of basis: $\log_a b = \frac{\log_c b}{\log_c a}$. Product Rule: $\log_a (b \cdot c) = \log_a b + \log_a c$.

Quotient Rule: $\log_a \left(\frac{b}{c}\right) = \log_a b - \log_a c$. Power Rule: $\log_a (b^n) = n \log_a b$

Trigonometry:

Basic definitions: $\tan \alpha = \frac{\sin \alpha}{\cos \alpha}$, $\cot \alpha = \frac{\cos \alpha}{\sin \alpha} = \frac{1}{\tan \alpha}$, $\sec \alpha = \frac{1}{\cos \alpha}$, $\csc \alpha = \frac{1}{\sin \alpha}$

Basic properties: $\sin(-\alpha) = -\sin \alpha$ $\cos(-\alpha) = \cos \alpha$ $\sin\left(\frac{\pi}{2} \pm \alpha\right) = \cos \alpha$

Periodicity: $\sin(\alpha + 2\pi) = \sin \alpha$ $\cos(\alpha + 2\pi) = \cos \alpha$ $\tan(\alpha + \pi) = \tan \alpha$

Pythagorean Theorem: $\sin^2 \alpha + \cos^2 \alpha = 1$ $1 + \tan^2 \alpha = \frac{1}{\cos^2 \alpha}$

Sum of angles: $\sin(\alpha \pm \beta) = \sin \alpha \cdot \cos \beta \pm \cos \alpha \cdot \sin \beta$
 $\cos(\alpha \pm \beta) = \cos \alpha \cos \beta \mp \sin \alpha \sin \beta$
 $\tan(\alpha \pm \beta) = \frac{\tan \alpha \pm \tan \beta}{1 \mp \tan \alpha \cdot \tan \beta}$

Double Angles:

$$\sin 2\alpha = 2 \sin \alpha \cdot \cos \alpha \quad \cos 2\alpha = \cos^2 \alpha - \sin^2 \alpha \quad \tan(2\alpha) = \frac{2 \tan \alpha}{1 - \tan^2 \alpha}$$

$$\cos 2\alpha = 2 \cos^2 \alpha - 1 \quad \cos 2\alpha = 1 - 2 \sin^2 \alpha$$

$$\sin^2 \alpha = \frac{1}{2}(1 - \cos 2\alpha) \quad \cos^2 \alpha = \frac{1}{2}(1 + \cos 2\alpha) \quad \tan \alpha = \frac{1 - \cos 2\alpha}{\sin 2\alpha} = \frac{\sin 2\alpha}{1 + \cos 2\alpha}$$

Products of sines and cosines:

$$\cos \alpha \cdot \sin \beta = \frac{1}{2}[\sin(\alpha + \beta) - \sin(\alpha - \beta)], \quad \sin \alpha \cdot \cos \beta = \frac{1}{2}[\sin(\alpha + \beta) + \sin(\alpha - \beta)]$$

$$\sin \alpha \cdot \sin \beta = \frac{1}{2}[\cos(\alpha - \beta) - \cos(\alpha + \beta)], \quad \cos \alpha \cdot \cos \beta = \frac{1}{2}[\cos(\alpha - \beta) + \cos(\alpha + \beta)]$$

Sums and Differences of sines, cosines:

$$\sin \alpha + \sin \beta = 2 \sin \frac{\alpha + \beta}{2} \cos \frac{\alpha - \beta}{2}, \quad \sin \alpha - \sin \beta = 2 \sin \frac{\alpha - \beta}{2} \cos \frac{\alpha + \beta}{2}$$

$$\cos \alpha + \cos \beta = 2 \cos \frac{\alpha + \beta}{2} \cos \frac{\alpha - \beta}{2}, \quad \cos \alpha - \cos \beta = -2 \sin \frac{\alpha - \beta}{2} \sin \frac{\alpha + \beta}{2}$$

Solving Equations:

$$\sin x = a \quad (\text{for } -1 \leq a \leq 1) \Rightarrow x = \arcsin a + 2\pi \cdot n \quad \text{or} \quad x = (\pi - \arcsin a) + 2\pi \cdot n$$

$$\cos x = a \quad (\text{for } -1 \leq a \leq 1) \Rightarrow x = \arccos a + 2\pi \cdot n \quad \text{or} \quad x = -\arccos a + 2\pi \cdot n$$

$$\tan x = a \quad (\text{for } -\infty < a < \infty) \Rightarrow x = \arctan a + \pi \cdot n$$

Triangles

The area of a triangle is $S = \frac{1}{2}h \cdot a$ (half height times base), or $S = \frac{1}{2}a \cdot b \cdot \sin \gamma$.

An inscribed angle in a circle is equal to half to central angle intercepting the same arc.

$$\text{Law of Sines: } \frac{a}{\sin \alpha} = \frac{b}{\sin \beta} = \frac{c}{\sin \gamma} = 2R.$$

$$\text{Law of Cosines: } c^2 = a^2 + b^2 - 2ab \cos \gamma.$$

Analytic Geometry

Distance between points (x_1, y_1) and (x_2, y_2) : $d = \sqrt{(x_2 - x_1)^2 + (y_2 - y_1)^2}$.

Equation of a line: $y = mx + n$ or $ax + by + c = 0$.

Equation of a line through the point (x_1, y_1) with slope m : $y - y_1 = m(x - x_1)$.

Slope of a line through the points (x_1, y_1) and (x_2, y_2) : $m = \left(\frac{y_2 - y_1}{x_2 - x_1} \right)$.

Slope of a line perpendicular to a line of slope m (for $(m \neq 0)$) is: $\left(-\frac{1}{m} \right)$.

Equation of a circle with radius R and center (a, b) : $(x - a)^2 + (y - b)^2 = R^2$.

Sequences

Arithmetic sequence: $a_n = a_1 + (n - 1)d$ ($n = 1, 2, \dots$); also $a_{n+1} = a_n + d$.

Sum formula of an arithmetic sequence: $S_n = a_1 + a_2 + \dots + a_n = (a_1 + a_n) \cdot \frac{n}{2}$

Geometric sequence: $a_n = a_1 \cdot q^{(n-1)}$ ($n = 1, 2, \dots$); also $a_{n+1} = a_n \cdot q$.

Sum formula of a geometric sequence: $S_n = a_1 + a_2 + \dots + a_n = \frac{a_1 \cdot (1 - q^n)}{1 - q}$

Sum formula of an infinite geometric sequence: $S = \frac{a_1}{1 - q}$, when $-1 < q < 1$.

Sets

Distributive laws: $A \cap (B \cup C) = (A \cap B) \cup (A \cap C)$, $A \cup (B \cap C) = (A \cup B) \cap (A \cup C)$

Complement: $A^c = \Omega - A$. De Morgan's laws: $(A \cap B)^c = A^c \cup B^c$, $(A \cup B)^c = A^c \cap B^c$

Basic Functions and Graphs

First degree function: $y = f(x) = mx + n$. Graph is a straight line.

Second degree function: $y = f(x) = ax^2 + bx + c$. Graph is a parabola.

If $f(-x) = f(x)$ then f is called even. If $f(-x) = -f(x)$ then f is called odd.

Composition of functions: $(f \circ g)(x) = f(g(x))$.

Inverse function: $y = f^{-1}(x)$. Satisfies: $(f \circ f^{-1})(x) = f(f^{-1}(x)) = x$.

Binomial Theorem: $(a + b)^n = a^n + na^{n-1}b + \dots + \binom{n}{k} a^{n-k} b^k + \dots + nab^{n-1} + b^n = \sum_{k=0}^n \binom{n}{k} a^{n-k} b^k$

(Term in position $k + 1$ is $\binom{n}{k} a^{n-k} b^k$, where $\binom{n}{k} = {}_n C_k = \frac{n!}{k!(n-k)!}$.)